src/Ex/Mesi.v
@@ -18,8 +18,6 @@ Definition mesiRsM: IdxT := 1~>3.
 Definition mesiDownRqI: IdxT := 1~>4.
 Definition mesiDownRsI: IdxT := 1~>5.
 
-Definition mesiPushRq: IdxT := 2~>2.
-Definition mesiPushWRq: IdxT := 2~>3.
 Definition mesiInvRq: IdxT := 2~>4.
 Definition mesiInvWRq: IdxT := 2~>5.
 Definition mesiInvRs: IdxT := 2~>6.
